Done 1st attempt page table abstraction for v/paddrs; TODO update example

proof/infoflow/timeprotection/TimeProtection.thy
@@ -212,20 +212,29 @@ locale time_protection =
     "\<And>s vas. touched_addrs (do_add_to_TA s vas) = touched_addrs s \<union> vas"
     "\<And>s vas. current_domain (do_add_to_TA s vas) = current_domain s"
     "\<And>s vas. v_to_p (do_add_to_TA s vas) = v_to_p s"
-  assumes do_add_to_TA_maintains_external_uwr: (* What a pain. This is all because
-    we aren't distinguishing touched_addresses from the rest of other_state -robs. *)
-    "\<And>s t vas.
+  assumes do_add_to_TA_maintains_external_uwr_in:
+    "\<And>s t d vas.
        (s, t) \<in> external_uwr d \<Longrightarrow>
+       current_domain s = d \<Longrightarrow>
        (do_add_to_TA s vas, do_add_to_TA t vas) \<in> external_uwr d"
+  assumes do_add_to_TA_maintains_external_uwr_out:
+    "\<And>s vas.
+       current_domain s \<noteq> d \<Longrightarrow>
+       (s, do_add_to_TA s vas) \<in> external_uwr d"
   fixes do_empty_TA :: "'other_state \<Rightarrow> 'other_state"
   assumes do_empty_TA_correct:
     "\<And>s. touched_addrs (do_empty_TA s) = {}"
     "\<And>s. current_domain (do_empty_TA s) = current_domain s"
     "\<And>s. v_to_p (do_empty_TA s) = v_to_p s"
-  assumes do_empty_TA_maintains_external_uwr:
-    "\<And>s t.
+  assumes do_empty_TA_maintains_external_uwr_in:
+    "\<And>s t d.
        (s, t) \<in> external_uwr d \<Longrightarrow>
+       current_domain s = d \<Longrightarrow>
        (do_empty_TA s, do_empty_TA t) \<in> external_uwr d"
+  assumes do_empty_TA_maintains_external_uwr_out:
+    "\<And>s.
+       current_domain s \<noteq> d \<Longrightarrow>
+       (s, do_empty_TA s) \<in> external_uwr d"
 
   (* We expect this to be true for, say, seL4's KSched \<rightarrow> KExit step. -robs. *)
   fixes can_domain_switch :: "'other_state \<Rightarrow> bool"
@@ -302,10 +311,15 @@ abbreviation touched_addrs' ::
   where
   "touched_addrs' s \<equiv> touched_addrs (other_state s)"
 
+definition paddrs_of ::
+  "'other_state \<Rightarrow> vaddr set \<Rightarrow> paddr set"
+  where
+  "paddrs_of s vas \<equiv> {a. \<exists>v. a = v_to_p s v \<and> v \<in> vas}"
+
 definition touched_paddrs ::
   "'other_state \<Rightarrow> paddr set"
   where
-  "touched_paddrs s \<equiv> {a. \<exists>v. a = v_to_p s v \<and> v \<in> touched_addrs s}"
+  "touched_paddrs s \<equiv> paddrs_of s (touched_addrs s)"
 
 abbreviation touched_paddrs' ::
   "('fch,'pch,'regs,'other_state)state \<Rightarrow> paddr set"
@@ -533,6 +547,7 @@ definition
   instrs_safe :: "'other_state \<Rightarrow> 'regs instr set" where
  "instrs_safe s \<equiv> {i. case i of
                     IWrite a \<Rightarrow> v_to_p s a \<notin> kernel_shared_precise
+                  | IAddToTA vas \<Rightarrow> paddrs_of s vas \<subseteq> all_addrs_of (current_domain s) \<union> kernel_shared_precise
                   | IEmptyTA \<Rightarrow> False
                   | _ \<Rightarrow> True}"
 
@@ -589,10 +604,12 @@ lemma safe_remains_safe:
   "i \<in> instrs_safe (other_state s) \<Longrightarrow>
    a \<in> instrs_safe (other_state s) \<Longrightarrow>
    i \<in> instrs_safe (other_state (instr_step a s))"
-  apply (cases i; cases a; clarsimp simp: instrs_safe_def)
-   using page_table_not_in_mem apply force
-  using do_add_to_TA_correct apply force
-  done
+  apply (cases i; cases a; clarsimp simp: instrs_safe_def all_addrs_of_def paddrs_of_def)
+     using page_table_not_in_mem apply force
+    using do_add_to_TA_correct apply force
+   using do_write_outside_kernelshared_same_domain kernel_shared_precise_def page_table_not_in_mem
+   apply auto[1]
+  using do_add_to_TA_correct(2) do_add_to_TA_correct(3) by auto
 
 lemma no_domainswitch_inv:
   "p \<in> programs_safe (other_state s) \<Longrightarrow>
@@ -685,6 +702,7 @@ lemma and_or_specific:
 lemma d_running_step:
   assumes
     "i \<in> instrs_obeying_ta (other_state s)"
+    "i \<in> instrs_safe (other_state s)"
     "touched_addrs_inv (other_state s)"
     "page_table_inv (other_state s)"
     "(s, t) \<in> uwr d"
@@ -706,7 +724,7 @@ lemma d_running_step:
       apply(clarsimp simp:all_addrs_of_def)
       apply(erule_tac x=a in allE)
       apply(erule_tac c="v_to_p' s a" in subsetCE)
-       apply(force simp:touched_paddrs_def)
+       apply(force simp:touched_paddrs_def paddrs_of_def)
       apply clarsimp
       apply(rule conjI)
        (* equivalence on part of pch *)
@@ -761,7 +779,7 @@ lemma d_running_step:
       apply(clarsimp simp:all_addrs_of_def)
       apply(erule_tac x=a in allE)
       apply(erule_tac c="v_to_p' s a" in subsetCE)
-       apply(force simp:touched_paddrs_def)
+       apply(force simp:touched_paddrs_def paddrs_of_def)
       apply clarsimp
       apply(rule conjI)
        (* equivalence on part of pch *)
@@ -814,11 +832,11 @@ lemma d_running_step:
         apply clarsimp
         apply (drule_tac x=a1 in spec)
         apply clarsimp
-        (* Adapted from an Isar proof -robs. *)
+        (* Adapted from an Isar proof found by Sledgehammer -robs. *)
         apply(prop_tac "full_collision_set {p. \<exists>pa. pa \<in> kernel_shared_precise \<and> p \<in> collision_set pa}")
          apply(metis (no_types) kernel_shared_expanded_def kernel_shared_expanded_full_collision_set)
         apply(prop_tac "fa \<subseteq> {v_to_p' s v |v. v \<in> touched_addrs' s}")
-         apply(force simp:touched_paddrs_def)
+         apply(force simp:touched_paddrs_def paddrs_of_def)
         apply(prop_tac "addr_domain a2 \<noteq> current_domain' s")
          apply(metis (no_types) diff_domain_no_collision)
         apply(prop_tac "addr_domain a2 = Sched")
@@ -852,15 +870,59 @@ lemma d_running_step:
     case (IAddToTA vas)
     thus ?thesis using assms
       apply(clarsimp simp:uwr_def uwr_running_def)
-      using do_add_to_TA_maintains_external_uwr
+      using do_add_to_TA_maintains_external_uwr_in
       by blast
   next
-    case (IEmptyTA)
+    case IEmptyTA
     thus ?thesis using assms
-      apply(clarsimp simp:uwr_def uwr_running_def)
-      using do_empty_TA_maintains_external_uwr
-      by blast
+      by (clarsimp simp:uwr_def uwr_running_def instrs_safe_def)
   qed
+
+lemma touched_addrs_inv_preserved:
+  "\<lbrakk>touched_addrs_inv' s; page_table_inv' s;
+    s' = instr_multistep p (instr_step a s);
+    current_domain' (instr_step a s) = current_domain' s;
+    a \<in> instrs_safe (other_state s)\<rbrakk>
+   \<Longrightarrow> touched_addrs_inv' (instr_step a s)"
+  apply(clarsimp simp:instrs_obeying_ta_def
+    programs_safe_def instrs_safe_def list_all_def split:instr.splits)
+   using page_table_inv_def page_table_not_in_mem touched_addrs_inv_def touched_paddrs_def paddrs_of_def
+   apply(force simp add: touched_addrs_not_in_mem)
+  using do_add_to_TA_correct(3) page_table_inv_def touched_addrs_inv_def touched_paddrs_def paddrs_of_def
+  apply auto[1]
+  done
+
+lemma touched_addrs_inv_preserved':
+  "\<lbrakk>a # p \<in> programs_obeying_ta (other_state s); a # p \<in> programs_safe (other_state s);
+    touched_addrs_inv' s; page_table_inv' s; (s, t) \<in> uwr (current_domain' s);
+    s' = instr_multistep p (instr_step a s); t' = instr_multistep p (instr_step a t);
+    d = current_domain' s; current_domain' (instr_step a s) = d\<rbrakk>
+   \<Longrightarrow> touched_addrs_inv' (instr_step a s)"
+  apply(clarsimp simp:programs_obeying_ta_def programs_safe_def)
+  using touched_addrs_inv_preserved by blast
+
+lemma page_table_inv_preserved:
+  "\<lbrakk>touched_addrs_inv' s; page_table_inv' s;
+    s' = instr_multistep p (instr_step a s);
+    current_domain' (instr_step a s) = current_domain' s;
+    a \<in> instrs_safe (other_state s)\<rbrakk>
+   \<Longrightarrow> page_table_inv' (instr_step a s)"
+  apply(clarsimp simp:programs_obeying_ta_def instrs_obeying_ta_def
+    programs_safe_def instrs_safe_def list_all_def split:instr.splits)
+   using page_table_inv_def page_table_not_in_mem touched_addrs_inv_def touched_paddrs_def
+   apply force
+  using do_add_to_TA_correct(3) page_table_inv_def touched_addrs_inv_def touched_paddrs_def
+  apply force
+  done
+
+lemma page_table_inv_preserved':
+  "\<lbrakk>a # p \<in> programs_obeying_ta (other_state s); a # p \<in> programs_safe (other_state s);
+    touched_addrs_inv' s; page_table_inv' s; (s, t) \<in> uwr (current_domain' s);
+    s' = instr_multistep p (instr_step a s); t' = instr_multistep p (instr_step a t);
+    d = current_domain' s; current_domain' (instr_step a s) = d\<rbrakk>
+   \<Longrightarrow> page_table_inv' (instr_step a s)"
+  apply(clarsimp simp:programs_obeying_ta_def programs_safe_def)
+  using page_table_inv_preserved by blast
 
 (* d running \<rightarrow> d running *)
 lemma d_running: "\<lbrakk>
@@ -893,35 +955,52 @@ lemma d_running: "\<lbrakk>
   apply clarsimp
   apply(erule meta_impE)
    apply(clarsimp simp:programs_obeying_ta_def instrs_obeying_ta_def list_all_def split:instr.splits)
-     apply(force simp add:touched_paddrs_def page_table_not_in_mem touched_addrs_not_in_mem)
-    unfolding touched_paddrs_def
+     apply(force simp add:touched_paddrs_def paddrs_of_def page_table_not_in_mem touched_addrs_not_in_mem)
+    unfolding touched_paddrs_def paddrs_of_def
     using do_add_to_TA_correct(1,3)
     apply clarsimp
     apply blast
    apply(force simp:programs_safe_def instrs_safe_def)
   apply(erule meta_impE)
    apply(clarsimp simp: programs_safe_def instrs_safe_def list_all_def split:instr.splits)
-    apply(force simp add:page_table_not_in_mem)
-   using do_add_to_TA_correct(3) apply auto[1]
+    (* Isar proof found by sledgehammer -robs. *)
+    subgoal proof -
+      fix pa :: "'regs instr list" and sa :: "('fch, 'pch, 'regs, 'other_state) state" and ta :: "('fch, 'pch, 'regs, 'other_state) state" and x2 :: vaddr and x :: "'regs instr"
+      assume a1: "\<forall>x\<in>set pa. (\<forall>x2. x = IWrite x2 \<longrightarrow> v_to_p' sa x2 \<notin> kernel_shared_precise) \<and> (\<forall>x8. x = IAddToTA x8 \<longrightarrow> paddrs_of (other_state sa) x8 \<subseteq> all_addrs_of (current_domain' sa) \<union> kernel_shared_precise) \<and> x \<noteq> IEmptyTA"
+      assume a2: "x \<in> set pa"
+      assume a3: "page_table_inv' sa"
+      assume a4: "v_to_p' sa x2 \<notin> kernel_shared_precise"
+      obtain vv :: vaddr and VV :: "vaddr set" where
+        f5: "((\<exists>v. x = IWrite v \<and> v_to_p (do_write x2 (other_state sa) (regs sa)) v \<in> kernel_shared_precise) \<or> (\<exists>V. x = IAddToTA V \<and> \<not> paddrs_of (do_write x2 (other_state sa) (regs sa)) V \<subseteq> all_addrs_of (current_domain (do_write x2 (other_state sa) (regs sa))) \<union> kernel_shared_precise)) = (x = IWrite vv \<and> v_to_p (do_write x2 (other_state sa) (regs sa)) vv \<in> kernel_shared_precise \<or> x = IAddToTA VV \<and> \<not> paddrs_of (do_write x2 (other_state sa) (regs sa)) VV \<subseteq> all_addrs_of (current_domain (do_write x2 (other_state sa) (regs sa))) \<union> kernel_shared_precise)"
+        by moura
+      obtain pp :: "paddr set \<Rightarrow> paddr set \<Rightarrow> paddr" where
+        "\<forall>x0 x1. (\<exists>v2. v2 \<in> x1 \<and> v2 \<notin> x0) = (pp x0 x1 \<in> x1 \<and> pp x0 x1 \<notin> x0)"
+        by moura
+      then have f6: "\<forall>P Pa. pp Pa P \<in> P \<and> pp Pa P \<notin> Pa \<or> P \<subseteq> Pa"
+        by (meson subsetI)
+      obtain vva :: "paddr \<Rightarrow> vaddr set \<Rightarrow> 'other_state \<Rightarrow> vaddr" where
+        "\<forall>x0 x1 x2a. (\<exists>v3. x0 = v_to_p x2a v3 \<and> v3 \<in> x1) = (x0 = v_to_p x2a (vva x0 x1 x2a) \<and> vva x0 x1 x2a \<in> x1)"
+        by moura
+      then have f7: "pp (all_addrs_of (current_domain (do_write x2 (other_state sa) (regs sa))) \<union> kernel_shared_precise) (paddrs_of (do_write x2 (other_state sa) (regs sa)) VV) \<in> paddrs_of (do_write x2 (other_state sa) (regs sa)) VV \<and> pp (all_addrs_of (current_domain (do_write x2 (other_state sa) (regs sa))) \<union> kernel_shared_precise) (paddrs_of (do_write x2 (other_state sa) (regs sa)) VV) \<notin> all_addrs_of (current_domain (do_write x2 (other_state sa) (regs sa))) \<union> kernel_shared_precise \<longrightarrow> pp (all_addrs_of (current_domain (do_write x2 (other_state sa) (regs sa))) \<union> kernel_shared_precise) (paddrs_of (do_write x2 (other_state sa) (regs sa)) VV) = v_to_p (do_write x2 (other_state sa) (regs sa)) (vva (pp (all_addrs_of (current_domain (do_write x2 (other_state sa) (regs sa))) \<union> kernel_shared_precise) (paddrs_of (do_write x2 (other_state sa) (regs sa)) VV)) VV (do_write x2 (other_state sa) (regs sa))) \<and> vva (pp (all_addrs_of (current_domain (do_write x2 (other_state sa) (regs sa))) \<union> kernel_shared_precise) (paddrs_of (do_write x2 (other_state sa) (regs sa)) VV)) VV (do_write x2 (other_state sa) (regs sa)) \<in> VV"
+        by (simp add: paddrs_of_def)
+      have "addr_domain (v_to_p' sa x2) \<noteq> Sched"
+        using a4 by (simp add: kernel_shared_precise_def)
+      then have "current_domain (do_write x2 (other_state sa) (regs sa)) = current_domain' sa"
+        by (meson time_protection.do_write_outside_kernelshared_same_domain time_protection_axioms)
+      then show "(\<forall>v. x = IWrite v \<longrightarrow> v_to_p (do_write x2 (other_state sa) (regs sa)) v \<notin> kernel_shared_precise) \<and> (\<forall>V. x = IAddToTA V \<longrightarrow> paddrs_of (do_write x2 (other_state sa) (regs sa)) V \<subseteq> all_addrs_of (current_domain (do_write x2 (other_state sa) (regs sa))) \<union> kernel_shared_precise)"
+        using f7 f6 f5 a3 a2 a1 by (metis (no_types) page_table_inv_def page_table_not_in_mem)
+    qed
+   apply(force simp add: do_add_to_TA_correct(2) do_add_to_TA_correct(3) paddrs_of_def)
   apply (subgoal_tac "current_domain' (instr_step a s) = d")
-   (* FIXME: Should probably prove this as a lemma for touched_addrs_inv *)
    apply (erule meta_impE)
-    apply(clarsimp simp:programs_obeying_ta_def instrs_obeying_ta_def list_all_def split:instr.splits)
-      using page_table_inv_def page_table_not_in_mem touched_addrs_inv_def touched_paddrs_def
-      apply force
-     using do_add_to_TA_correct(3) page_table_inv_def touched_addrs_inv_def touched_paddrs_def
-     apply force
-    apply(force simp add:do_empty_TA_correct(1) touched_addrs_inv_def touched_paddrs_def)
-   (* FIXME: Should probably prove this as a lemma for page_table_inv *)
+    apply(clarsimp simp:programs_obeying_ta_def programs_safe_def)
+    using touched_addrs_inv_preserved
+    apply blast
    apply (erule meta_impE)
-   apply(clarsimp simp:programs_obeying_ta_def instrs_obeying_ta_def list_all_def split:instr.splits)
-     using page_table_inv_def page_table_not_in_mem touched_addrs_inv_def touched_paddrs_def
-     apply force
-    using do_add_to_TA_correct(3) page_table_inv_def touched_addrs_inv_def touched_paddrs_def
-    apply force
-   apply(force simp add: do_empty_TA_correct(3) page_table_inv_def)
-   apply clarsimp
-   apply(fastforce dest:d_running_step)
+    apply(clarsimp simp:programs_obeying_ta_def programs_safe_def)
+    using page_table_inv_preserved
+    apply blast
+   apply(metis (no_types, lifting) d_running_step hd_instr_obeying_ta list_all_simps(1) mem_Collect_eq time_protection.programs_safe_def time_protection_axioms)
   using safe_no_domainswitch
   apply (metis list_all_simps(1) mem_Collect_eq programs_safe_def)
   done
@@ -929,13 +1008,12 @@ lemma d_running: "\<lbrakk>
 
 
 
-(* DOWN TO HERE -robs.
-
 lemma d_not_running_step:
   assumes
-  "i \<in> instrs_obeying_ta ta"
-  "i \<in> instrs_safe"
-  "ta \<inter> all_addrs_of d = {}"
+  "i \<in> instrs_obeying_ta (other_state s)"
+  "i \<in> instrs_safe (other_state s)"
+  "touched_addrs_inv' s"
+  "page_table_inv' s"
   "current_domain' s \<noteq> d"
   "s' = instr_step i s"
   shows
@@ -946,26 +1024,32 @@ lemma d_not_running_step:
       apply (clarsimp simp: uwr_def uwr_notrunning_def pch_same_for_domain_except_shared_def
                             instrs_obeying_ta_def)
       (* show that the instruction hasn't affected our visible part of pch *)
-      apply (drule(1) in_inter_empty)
+      apply (drule in_inter_empty)
+       apply force
       apply (clarsimp simp: all_addrs_of_def)
       apply (rule pch_partitioned_read, clarsimp)
-      apply (erule(1) diff_domain_no_collision, simp)
-      done
+      using diff_domain_no_collision
+      by (metis (mono_tags, lifting) Un_iff all_addrs_of_def collision_sym
+        kernel_shared_expanded_def mem_Collect_eq page_table_inv_def)
   next
     case (IWrite x2)
     then show ?thesis using assms
       apply (clarsimp simp: uwr_def uwr_notrunning_def pch_same_for_domain_except_shared_def
                             instrs_obeying_ta_def)
       apply (thin_tac "s' = _")
-      apply (drule(1) in_inter_empty)
+      apply (drule in_inter_empty)
+       apply force
       apply (intro conjI)
        apply (clarsimp simp: all_addrs_of_def)
        apply (rule pch_partitioned_write, clarsimp)
-       apply (erule(1) diff_domain_no_collision, simp)
+       using diff_domain_no_collision
+       apply (metis (mono_tags, lifting) Un_iff all_addrs_of_def collision_sym
+         kernel_shared_expanded_def mem_Collect_eq page_table_inv_def)
       apply (rule do_write_maintains_external_uwr_out)
       apply (clarsimp simp: all_addrs_of_def)
       apply (clarsimp simp: instrs_safe_def kernel_shared_precise_def)
-      done
+      by (metis (mono_tags) Un_iff all_addrs_of_def kernel_shared_precise_def mem_Collect_eq
+        page_table_inv_def)
   next
     case (IRegs x3)
     then show ?thesis using assms
@@ -980,10 +1064,15 @@ lemma d_not_running_step:
       apply (clarsimp simp: uwr_def uwr_notrunning_def pch_same_for_domain_except_shared_def
                             instrs_obeying_ta_def)
       apply (rule sym, rule pch_partitioned_flush, clarsimp)
-      apply (drule(2) in_sub_inter_empty)
-      apply (thin_tac "s' = _") (* just clearing junk *)
-      apply (clarsimp simp: all_addrs_of_def)
-      apply (erule(2) diff_domain_no_collision)
+      apply(clarsimp simp:touched_addrs_inv_def all_addrs_of_def)
+      (* Adapted from Isar proof found by Sledgehammer -robs. *)
+      apply(prop_tac "addr_domain a' = d")
+       using diff_domain_no_collision
+       apply blast
+      apply(prop_tac "a \<in> kernel_shared_precise")
+       apply(force simp:kernel_shared_precise_def)
+      using collision_set_contains_itself kernel_shared_expanded_def
+      apply blast
       done
   next
     case IReadTime
@@ -993,6 +1082,17 @@ lemma d_not_running_step:
     case (IPadToTime x7)
     then show ?thesis using assms
       by (clarsimp simp: uwr_def uwr_notrunning_def pch_same_for_domain_except_shared_def)
+  next
+    case (IAddToTA vas)
+    thus ?thesis using assms
+      apply(clarsimp simp: uwr_def uwr_notrunning_def pch_same_for_domain_except_shared_def)
+      using do_add_to_TA_maintains_external_uwr_out
+      by blast
+  next
+    case IEmptyTA
+    thus ?thesis using assms
+      by (clarsimp simp: uwr_def uwr_notrunning_def pch_same_for_domain_except_shared_def
+        instrs_safe_def)
 qed
 
 
@@ -1004,16 +1104,18 @@ lemma programs_obeying_ta_head_and_rest:
   done
 
 lemma programs_safe_head_and_rest:
-  "h # r \<in> programs_safe \<Longrightarrow>
-   h \<in> instrs_safe \<and> r \<in> programs_safe"
+  "h # r \<in> programs_safe s \<Longrightarrow>
+   h \<in> instrs_safe s \<and> r \<in> programs_safe s"
   apply (clarsimp simp: programs_safe_def)
   done                          
 
 lemma d_not_running_integrity_uwr:
-  "\<lbrakk>p \<in> programs_obeying_ta ta;
-  p \<in> programs_safe; 
+  "\<lbrakk>p \<in> programs_obeying_ta (other_state s);
+  p \<in> programs_safe (other_state s);
   current_domain' s \<noteq> d;
-  ta \<inter> all_addrs_of d = {} \<rbrakk> \<Longrightarrow>
+  touched_addrs_inv' s;
+  page_table_inv' s
+  \<rbrakk> \<Longrightarrow>
   (s, instr_multistep p s) \<in> uwr d"
   apply (induct p arbitrary: s; clarsimp)
   apply (drule programs_obeying_ta_head_and_rest, clarsimp)
@@ -1022,27 +1124,72 @@ lemma d_not_running_integrity_uwr:
    defer
    using safe_no_domainswitch
    apply blast
+  unfolding programs_obeying_ta_def programs_safe_def
   apply (drule_tac x="instr_step a s" in meta_spec)
+  apply(erule meta_impE)
+   apply(clarsimp simp:instrs_obeying_ta_def instrs_safe_def list_all_def split:instr.splits)
+    using page_table_not_in_mem touched_paddrs_def
+    apply(force simp add: touched_addrs_not_in_mem paddrs_of_def)
+   (* Isar proof found by Sledgehammer -robs. *)
+   subgoal
+   proof -
+     fix pa :: "'regs instr list" and sa :: "('fch, 'pch, 'regs, 'other_state) state" and x8 :: "vaddr set" and x :: "'regs instr"
+     assume a1: "\<forall>x\<in>set pa. (\<forall>x1. x = IRead x1 \<longrightarrow> x1 \<in> touched_addrs' sa) \<and> (\<forall>x2. x = IWrite x2 \<longrightarrow> x2 \<in> touched_addrs' sa) \<and> (\<forall>x5. x = IFlushL2 x5 \<longrightarrow> x5 \<subseteq> touched_paddrs' sa)"
+     assume a2: "x \<in> set pa"
+     have f3: "((\<forall>v. x = IRead v \<longrightarrow> v \<in> touched_addrs (do_add_to_TA (other_state sa) x8)) \<and> (\<forall>v. x = IWrite v \<longrightarrow> v \<in> touched_addrs (do_add_to_TA (other_state sa) x8)) \<and> (\<forall>P. x = IFlushL2 P \<longrightarrow> P \<subseteq> touched_paddrs (do_add_to_TA (other_state sa) x8))) = ((\<forall>v. x \<noteq> IRead v \<or> v \<in> touched_addrs (do_add_to_TA (other_state sa) x8)) \<and> (\<forall>v. x \<noteq> IWrite v \<or> v \<in> touched_addrs (do_add_to_TA (other_state sa) x8)) \<and> (\<forall>P. x \<noteq> IFlushL2 P \<or> P \<subseteq> touched_paddrs (do_add_to_TA (other_state sa) x8)))"
+       by presburger
+     obtain vv :: vaddr and vva :: vaddr and PP :: "paddr set" where
+       f4: "((\<exists>v. x = IRead v \<and> v \<notin> touched_addrs (do_add_to_TA (other_state sa) x8)) \<or> (\<exists>v. x = IWrite v \<and> v \<notin> touched_addrs (do_add_to_TA (other_state sa) x8)) \<or> (\<exists>P. x = IFlushL2 P \<and> \<not> P \<subseteq> touched_paddrs (do_add_to_TA (other_state sa) x8))) = (x = IRead vva \<and> vva \<notin> touched_addrs (do_add_to_TA (other_state sa) x8) \<or> x = IWrite vv \<and> vv \<notin> touched_addrs (do_add_to_TA (other_state sa) x8) \<or> x = IFlushL2 PP \<and> \<not> PP \<subseteq> touched_paddrs (do_add_to_TA (other_state sa) x8))"
+       by moura
+     obtain pp :: "paddr set \<Rightarrow> paddr set \<Rightarrow> paddr" where
+       f5: "\<forall>x0 x1. (\<exists>v2. v2 \<in> x1 \<and> v2 \<notin> x0) = (pp x0 x1 \<in> x1 \<and> pp x0 x1 \<notin> x0)"
+       by moura
+     have "x = IFlushL2 PP \<and> \<not> PP \<subseteq> touched_paddrs (do_add_to_TA (other_state sa) x8) \<longrightarrow> PP \<subseteq> {v_to_p' sa v |v. v \<in> touched_addrs' sa}"
+       using a2 a1 by (simp add: touched_paddrs_def paddrs_of_def)
+     then have f6: "x = IFlushL2 PP \<and> \<not> PP \<subseteq> touched_paddrs (do_add_to_TA (other_state sa) x8) \<longrightarrow> (\<exists>v. pp (touched_paddrs (do_add_to_TA (other_state sa) x8)) PP = v_to_p' sa v \<and> v \<in> touched_addrs' sa)"
+       using f5 by blast
+     have "x = IFlushL2 PP \<and> \<not> PP \<subseteq> touched_paddrs (do_add_to_TA (other_state sa) x8) \<longrightarrow> pp (touched_paddrs (do_add_to_TA (other_state sa) x8)) PP \<notin> {v_to_p (do_add_to_TA (other_state sa) x8) v |v. v \<in> touched_addrs (do_add_to_TA (other_state sa) x8)}"
+       using f5 by (metis subsetI touched_paddrs_def paddrs_of_def)
+     then show "(\<forall>v. x = IRead v \<longrightarrow> v \<in> touched_addrs (do_add_to_TA (other_state sa) x8)) \<and> (\<forall>v. x = IWrite v \<longrightarrow> v \<in> touched_addrs (do_add_to_TA (other_state sa) x8)) \<and> (\<forall>P. x = IFlushL2 P \<longrightarrow> P \<subseteq> touched_paddrs (do_add_to_TA (other_state sa) x8))"
+       using f6 f4 f3 a2 a1 do_add_to_TA_correct(1) do_add_to_TA_correct(3) by force
+   qed
+  apply(erule meta_impE)
+   apply(clarsimp simp:instrs_obeying_ta_def instrs_safe_def list_all_def split:instr.splits)
+    using page_table_not_in_mem touched_paddrs_def paddrs_of_def touched_addrs_not_in_mem
+    apply (force simp add: do_write_outside_kernelshared_same_domain kernel_shared_precise_def)
+   using do_add_to_TA_correct(3)
+   apply (force simp add: do_add_to_TA_correct(2) paddrs_of_def)
+  apply(erule meta_impE)
+   apply force
+  apply(erule meta_impE)
+   using touched_addrs_inv_preserved
+   apply(force simp add: safe_no_domainswitch)
+  apply(erule meta_impE)
+   using page_table_inv_preserved
+   apply(force simp add: safe_no_domainswitch)
   apply (rule_tac b="instr_step a s" in uwr_trans)
    defer
-   apply assumption 
+   apply assumption
   (* now we are down to the single step *)
-  apply (erule_tac i=a and ta=ta in d_not_running_step; simp)
+  defer
+  apply (erule_tac i=a in d_not_running_step; simp)
   done
 
 (* d not running \<rightarrow> d not running *)
 lemma d_not_running: "\<lbrakk>
    \<comment> \<open>we have two programs derived from touched_addresses - may not be the same touched_addresses\<close>
-   p\<^sub>s \<in> programs_obeying_ta ta\<^sub>s;
-   p\<^sub>t \<in> programs_obeying_ta ta\<^sub>t;   
-   p\<^sub>s \<in> programs_safe;
-   p\<^sub>t \<in> programs_safe;
+   p\<^sub>s \<in> programs_obeying_ta (other_state s);
+   p\<^sub>t \<in> programs_obeying_ta (other_state t);
+   p\<^sub>s \<in> programs_safe (other_state s);
+   p\<^sub>t \<in> programs_safe (other_state t);
    \<comment> \<open>we may not have concrete touched_addresses -
      we may overapprox this to the whole currently running domain.
      NB: I think it's enough just to require it not contain any of d's addresses. -robs.\<close>
    \<comment> \<open>these touched_addresses does NOT contain any addresses from d\<close>
-   ta\<^sub>s \<inter> all_addrs_of d = {};
-   ta\<^sub>t \<inter> all_addrs_of d = {};
+   touched_addrs_inv' s;
+   touched_addrs_inv' t;
+   page_table_inv' s;
+   page_table_inv' t;
    \<comment> \<open>initial states s and t hold uwr_notrunning\<close>
    (s, t) \<in> uwr d;
    current_domain' s \<noteq> d;
@@ -1057,8 +1204,8 @@ lemma d_not_running: "\<lbrakk>
    (s', t') \<in> uwr d"
   apply clarsimp
   apply (subgoal_tac "current_domain' t \<noteq> d")
-   apply (drule(3) d_not_running_integrity_uwr [where s=s])
-   apply (drule(3) d_not_running_integrity_uwr [where s=t])
+   apply (drule(4) d_not_running_integrity_uwr [where s=s])
+   apply (drule(4) d_not_running_integrity_uwr [where s=t])
   apply (rule uwr_trans, subst uwr_sym, assumption)
    apply (rule uwr_trans, assumption, assumption)
   using uwr_same_domain apply blast
@@ -1204,7 +1351,7 @@ definition
 
 
 
-
+(* XXX: Just commenting it out unchanged to avoid any nasty merge conflicts -robs.
 (*FIXME: This is a draft *)
 (* d running \<rightarrow> d not running *)
 lemma context_switch_from_d: "\<lbrakk>
@@ -1237,6 +1384,7 @@ lemma context_switch_to_d: "\<lbrakk>
    \<rbrakk> \<Longrightarrow>
    (s', t') \<in> uwr d"
   oops
+*)
 
 
 
@@ -1354,6 +1502,8 @@ lemma programs_obeying_ta_preserve_uwr: "\<lbrakk>
    \<not> can_domain_switch (other_state t);
    touched_addrs_inv' s;
    touched_addrs_inv' t;
+   page_table_inv' s;
+   page_table_inv' t;
    is_secure_nondomainswitch p\<^sub>s s;
    is_secure_nondomainswitch p\<^sub>t t;
    (s, t) \<in> uwr d;
@@ -1368,34 +1518,12 @@ lemma programs_obeying_ta_preserve_uwr: "\<lbrakk>
    apply clarsimp
    apply(prop_tac "current_domain' s' = d")
     apply(metis no_domainswitch_inv)
-   apply(rule d_running)
-        apply force
-       apply force
-      apply(force simp:touched_addrs_inv_def)
-     apply force
-    apply force
-   apply force
-  apply(frule uwr_same_touched_addrs)
-    apply force
-   apply force
+   apply(force intro:d_running)
   apply(prop_tac "current_domain' s' \<noteq> d")
    apply(metis no_domainswitch_inv)
   apply clarsimp
-  apply(rule d_not_running[where s=s and t=t and p\<^sub>s=p\<^sub>s and p\<^sub>t=p\<^sub>t and
-        ta\<^sub>s="touched_addrs' s" and ta\<^sub>t="touched_addrs' t"])
-            apply force
-           apply force
-          apply force
-         apply force
-        (* using touched_addrs_inv' *)
-        defer (* FIXME: Think more about these two. -robs. *)
-       defer
-      apply force
-     apply force
-    apply force
-   apply force
-  apply force
-  sorry
+  apply(force intro:d_not_running[where s=s and t=t and p\<^sub>s=p\<^sub>s and p\<^sub>t=p\<^sub>t])
+  done
 
 end
 
@@ -1478,7 +1606,7 @@ locale time_protection_refinement =
     fch_read_impact pch_read_impact fch_write_impact pch_write_impact
     read_cycles write_cycles do_read do_write store_time padding_regs_impact
     empty_fch fch_flush_cycles do_pch_flush pch_flush_cycles addr_domain addr_colour colour_userdomain
-    current_domain external_uwr touched_addrs can_domain_switch
+    current_domain external_uwr v_to_p touched_addrs do_add_to_TA do_empty_TA can_domain_switch
   for A :: "('a,'other_state,unit) data_type"
   and C :: "('c,'other_state,unit) data_type"
   and s0 :: "'other_state"
@@ -1486,32 +1614,37 @@ locale time_protection_refinement =
   and external_uwr :: "'userdomain domain \<Rightarrow> ('other_state \<times> 'other_state) set"
   and policy :: "('userdomain domain \<times> 'userdomain domain) set"
   and out :: "'userdomain domain \<Rightarrow> 'other_state \<Rightarrow> 'p"
-  and collides_in_pch :: "address rel"
+  and collides_in_pch :: "paddr rel"
   and fch_lookup :: "'fch \<Rightarrow> 'fch_cachedness fch"
   and pch_lookup :: "'pch \<Rightarrow> 'pch_cachedness pch"
   and fch_read_impact :: "'fch fch_impact"
-  and pch_read_impact :: "('fch, 'pch) pch_impact"
+  and pch_read_impact :: "'pch pch_impact"
   and fch_write_impact :: "'fch fch_impact"
-  and pch_write_impact :: "('fch, 'pch) pch_impact"
+  and pch_write_impact :: "'pch pch_impact"
   and read_cycles  :: "'fch_cachedness \<Rightarrow> 'pch_cachedness \<Rightarrow> time"
   and write_cycles :: "'fch_cachedness \<Rightarrow> 'pch_cachedness \<Rightarrow> time"
-  and do_read :: "address \<Rightarrow> 'other_state \<Rightarrow> 'regs \<Rightarrow> 'regs"
-  and do_write :: "address \<Rightarrow> 'other_state \<Rightarrow> 'regs \<Rightarrow> 'other_state"
+  and do_read :: "vaddr \<Rightarrow> 'other_state \<Rightarrow> 'regs \<Rightarrow> 'regs"
+  and do_write :: "vaddr \<Rightarrow> 'other_state \<Rightarrow> 'regs \<Rightarrow> 'other_state"
   and store_time :: "time \<Rightarrow> 'regs \<Rightarrow> 'regs"
   and padding_regs_impact :: "time \<Rightarrow> 'regs \<Rightarrow> 'regs"
   and empty_fch :: "'fch"
   and fch_flush_cycles :: "'fch \<Rightarrow> time"
-  and do_pch_flush :: "'pch \<Rightarrow> address set \<Rightarrow> 'pch"
-  and pch_flush_cycles :: "'pch \<Rightarrow> address set \<Rightarrow> time"
-  and addr_domain :: "address \<Rightarrow> 'userdomain domain"
-  and addr_colour :: "address \<Rightarrow> 'colour"
+  and do_pch_flush :: "'pch \<Rightarrow> paddr set \<Rightarrow> 'pch"
+  and pch_flush_cycles :: "'pch \<Rightarrow> paddr set \<Rightarrow> time"
+  and addr_domain :: "paddr \<Rightarrow> 'userdomain domain"
+  and addr_colour :: "paddr \<Rightarrow> 'colour"
   and colour_userdomain :: "'colour \<Rightarrow> 'userdomain"
-  and touched_addrs :: "'other_state \<Rightarrow> address set"
+  and v_to_p :: "'other_state \<Rightarrow> vaddr \<Rightarrow> paddr"
+  and touched_addrs :: "'other_state \<Rightarrow> vaddr set"
+  and do_add_to_TA :: "'other_state \<Rightarrow> vaddr set \<Rightarrow> 'other_state"
+  and do_empty_TA :: "'other_state \<Rightarrow> 'other_state"
   and can_domain_switch :: "'other_state \<Rightarrow> bool" +
   fixes initial_regs :: "'regs"
   fixes initial_pch :: "'pch"
   assumes A_touched_addrs_inv:
     "abs.reachable s \<Longrightarrow> touched_addrs_inv s"
+  assumes A_page_table_inv:
+    "abs.reachable s \<Longrightarrow> page_table_inv s"
   fixes C_step_program :: "'other_state \<Rightarrow> 'other_state \<Rightarrow> 'regs program"
   assumes reachable_C_nondomainswitch_reqs:
     "(\<And> s s' p.
@@ -1851,8 +1984,10 @@ theorem extended_confidentiality_u:
   apply(clarsimp simp:Let_def)
   apply(rename_tac u s t s_priv' s_priv t_priv' t_priv)
   apply(rule programs_obeying_ta_preserve_uwr, simp_all)
-    apply(force simp:A_touched_addrs_inv reachable)
-   apply(force simp:A_touched_addrs_inv reachable)
+      apply(force simp:A_touched_addrs_inv reachable)
+     apply(force simp:A_touched_addrs_inv reachable)
+    apply(force simp:A_page_table_inv reachable)
+   apply(force simp:A_page_table_inv reachable)
   apply(force simp:kludge_uwr_same_programs_def)
   done
 
